Modify problem0002 to print the answer

problem0002.v
@@ -3,12 +3,12 @@ Require Import ExtrOcamlNatInt.
 Require Import Bool Arith NPeano.
 Require Import Coq.Arith.Wf_nat.
 
-(* Program Fixpoint, Function *)
 
 Inductive fib_spec : nat -> nat -> Prop :=
 | fib_spec1 : fib_spec 0 1
 | fib_spec2 : fib_spec 1 2
 | fib_spec3 : forall i n m, fib_spec i n -> fib_spec (S i) m -> fib_spec (S (S i)) (n + m).
+
 
 Fixpoint fib (n:nat) : nat :=
   match n with
@@ -16,6 +16,7 @@ Fixpoint fib (n:nat) : nat :=
   | 1 => 2
   | S (S n'' as n') => fib n'' + fib n'
   end.
+
 
 Theorem fib_correct : forall i n, fib i = n <-> fib_spec i n.
 split.
@@ -69,7 +70,9 @@ split.
      assumption.
 Qed.
 
+
 Parameter bound : nat.
+
 
 Inductive spec_sub : nat -> nat -> Prop :=
 | spec_sub1 : spec_sub 0 0
@@ -83,7 +86,9 @@ Inductive spec_sub : nat -> nat -> Prop :=
   forall i n, spec_sub i n ->
     fib i >= bound -> spec_sub (S i) n.
 
+
 Definition spec (n:nat) : Prop := forall i, fib i > bound -> spec_sub i n.
+
 
 Theorem fib_invariant : forall n, fib n + fib (S n) = fib (S (S n)).
 destruct n.
@@ -95,12 +100,14 @@ destruct n.
   reflexivity.
 Qed.
 
+
 Fixpoint fib_fast_pre (a:nat) (b:nat) (n:nat) : nat :=
   match n with
   | O => a
   | S n' => fib_fast_pre b (a+b) n'
   end.
 Definition fib_fast := fib_fast_pre 1 2.
+
 
 Lemma fib_fast_pre_correct : forall a b n k,
   fib n = a ->
@@ -141,6 +148,7 @@ induction k; intros.
     assumption.
 Qed.
 
+
 Theorem fib_fast_correct : forall n, fib n = fib_fast n.
 Proof.
 intro n.
@@ -148,7 +156,9 @@ unfold fib_fast.
 rewrite fib_fast_pre_correct with 1 2 0 n; auto.
 Qed.
 
+
 Lemma fib_geq1 : forall n, 0 < fib n.
+Proof.
 induction n; auto.
 simpl.
 destruct n; auto.
@@ -157,7 +167,9 @@ apply le_plus_trans.
 assumption.
 Qed.
 
+
 Theorem fib_increase_S : forall n, fib n < fib (S n).
+Proof.
 intro n.
 destruct n; auto.
 rewrite<- fib_invariant.
@@ -168,7 +180,9 @@ apply add_lt_le_mono.
  constructor.
 Qed.
 
+
 Theorem fib_increase_le : forall n m, n <= m -> fib n <= fib m.
+Proof.
 intros n m; generalize dependent n.
 induction m.
  inversion 1.
@@ -188,6 +202,7 @@ induction m.
   subst.
   auto.
 Qed.
+
 
 Lemma sub_lt_sub : forall n m l, n > l -> l < m -> n - m < n - l.
 Proof.
@@ -235,73 +250,8 @@ induction n.
 Qed.
 
 
-Fixpoint ble_nat (n:nat) (m:nat) : bool :=
-  match n with
-  | O => true
-  | S n' =>
-    match m with
-    | O => false
-    | S m' => ble_nat n' m'
-    end
-  end.
-
-Theorem ble_nat_true : forall n m, ble_nat n m = true -> n <= m.
-induction n; intros.
- destruct m.
-  auto.
-
-  auto with arith.
-
- destruct m.
-  inversion H.
-
-  apply le_n_S.
-  apply IHn.
-  simpl in H.
-  assumption.
-Qed.
-
-Theorem ble_nat_false : forall n m, ble_nat n m = false -> n > m.
-induction n; intros.
- inversion H.
-
- destruct m.
-  auto with arith.
-
-  apply lt_n_S.
-  apply IHn.
-  simpl in H.
-  assumption.
-Qed.
-
-Function f (acc:nat) (n:nat) {measure (fun n => S bound - fib n) n} : nat :=
-  let x := fib n in
-    if ble_nat bound x
-    then acc
-    else
-      if beq_nat (x mod 2) 0
-      then f (acc+x) (S n)
-      else f acc (S n).
-intros.
-apply sub_lt_sub.
- apply lt_le_weak.
- apply lt_n_S.
- apply ble_nat_false.
- assumption.
-
- apply fib_increase_S.
-
-intros.
-apply sub_lt_sub.
- apply lt_le_weak.
- apply lt_n_S.
- apply ble_nat_false.
- assumption.
-
- apply fib_increase_S.
-Defined.
-
 Lemma spec_sub_inv_step : forall i n, fib i >= bound -> spec_sub i n -> spec_sub (S i) n.
+Proof.
 induction i; intros.
  inversion H0.
  apply spec_sub4.
@@ -315,7 +265,9 @@ induction i; intros.
   assumption.
 Qed.
 
+
 Lemma spec_sub_inv1 : forall i j n, fib i >= bound -> j >= i -> spec_sub i n -> spec_sub j n.
+Proof.
 induction j; intros.
  inversion H0.
  subst.
@@ -341,7 +293,9 @@ induction j; intros.
   assumption.
 Qed.
 
+
 Lemma spec_sub_inv2 : forall i j n, fib i >= bound -> j >= i -> spec_sub j n -> spec_sub i n.
+Proof.
 induction j; intros.
  inversion H0.
  subst.
@@ -384,7 +338,79 @@ destruct (le_ge_dec i j).
 Qed.
 
 
-Theorem f_correct : forall acc n, spec_sub n acc -> spec (f acc n).
+Fixpoint ble_nat (n:nat) (m:nat) : bool :=
+  match n with
+  | O => true
+  | S n' =>
+    match m with
+    | O => false
+    | S m' => ble_nat n' m'
+    end
+  end.
+
+
+Theorem ble_nat_true : forall n m, ble_nat n m = true -> n <= m.
+Proof.
+induction n; intros.
+ destruct m.
+  auto.
+
+  auto with arith.
+
+ destruct m.
+  inversion H.
+
+  apply le_n_S.
+  apply IHn.
+  simpl in H.
+  assumption.
+Qed.
+
+
+Theorem ble_nat_false : forall n m, ble_nat n m = false -> n > m.
+Proof.
+induction n; intros.
+ inversion H.
+
+ destruct m.
+  auto with arith.
+
+  apply lt_n_S.
+  apply IHn.
+  simpl in H.
+  assumption.
+Qed.
+
+
+Function f (acc:nat) (n:nat) {measure (fun n => S bound - fib n) n} : nat :=
+  let x := fib n in
+    if ble_nat bound x
+    then acc
+    else
+      if beq_nat (x mod 2) 0
+      then f (acc+x) (S n)
+      else f acc (S n).
+intros.
+apply sub_lt_sub.
+ apply lt_le_weak.
+ apply lt_n_S.
+ apply ble_nat_false.
+ assumption.
+
+ apply fib_increase_S.
+
+intros.
+apply sub_lt_sub.
+ apply lt_le_weak.
+ apply lt_n_S.
+ apply ble_nat_false.
+ assumption.
+
+ apply fib_increase_S.
+Defined.
+
+
+Theorem f_correct_sub : forall acc n, spec_sub n acc -> spec (f acc n).
 apply (f_ind (fun acc n m => spec_sub n acc -> spec m)); intros.
  unfold spec; intros.
  apply spec_sub_inv with n.
@@ -415,3 +441,19 @@ apply (f_ind (fun acc n m => spec_sub n acc -> spec m)); intros.
   apply ble_nat_false.
   assumption.
 Qed.
+
+Definition ans := f 0 0.
+
+Corollary ans_correct : spec ans.
+apply f_correct_sub.
+constructor.
+Qed.
+
+Definition print_int (n:nat) : unit := tt.
+Definition main : unit := print_int ans.
+
+Extract Constant modulo => "(mod)".
+Extract Constant ble_nat => "(<=)".
+Extract Constant print_int => "print_int".
+Extract Constant bound => "4_000_000".
+Extraction "problem0002.ml" main.
